Start of example on assume-guarantee.

lunarlander_sl/ext2/BigStepEx.thy
@@ -131,7 +131,7 @@ proof -
         valg s0 ''a'' X + 1" for s0::"'a gstate"
     by auto
   show ?thesis
-  (* Stage 1: merge ex2_c and ex2_c' *)
+  (* Stage 1: merge ex2a_sp and ex2b_sp *)
   apply (rule spec_of_global_post)
    apply (rule spec_of_parallel)
       apply (rule spec_of_single)
@@ -139,7 +139,7 @@ proof -
   apply (rule spec_of_single)
      apply (rule ex2b_sp)
     apply simp apply simp
-  (* Stage 2: rewrite the assertions*)
+  (* Stage 2: rewrite the assertions *)
   apply auto subgoal for s0
     apply (auto simp: single_assn_wait_in single_assn_wait_out updg_subst2 single_assn_init)
   (* Stage 3: combine the two assertions *)
@@ -469,7 +469,7 @@ lemma sync_gassn_ifg_left:
   apply auto
   subgoal for s tr
     apply (elim sync_gassn.cases) apply clarify
-    subgoal premises pre for s11 _ s12 _ s21 s22 _ tr1 _ tr2
+    subgoal premises pre for s11 _ s12 _ s21 s22 _ tr1 _ tr2 _ tr'
     proof (cases "b (the (s11 pn))")
       case True
       show ?thesis
@@ -734,5 +734,252 @@ lemma ex5:
   apply (rule exists_gassn_elim)
   apply (rule exists_gassn_elim)
   using ex5'' by auto
+
+subsubsection \<open>Example 6\<close>
+
+text \<open>This example tests unmatched communications, and
+  preliminary use of assume-guarantee.
+
+   ch2?X; wait(1); ch1!X
+|| wait(1); ch1?X
+
+  ch2?X receives value from a third process. Complications
+  would arise if it does not occur immediately. Hence we
+  assume that it does.
+\<close>
+
+definition ex6a :: "'a proc" where
+  "ex6a = (Cm (ch2[?]X); Wait (\<lambda>_. 1); Cm (ch1[!](\<lambda>s. val s X)))"
+
+text \<open>Waiting an amount of time, without state change\<close>
+inductive wait_c :: "'a eexp \<Rightarrow> 'a assn2 \<Rightarrow> 'a assn2" where
+  "e s0 > 0 \<Longrightarrow> P s0 s tr \<Longrightarrow> wait_c e P s0 s (WaitBlock (e s0) (\<lambda>_. s0) ({}, {}) # tr)"
+| "\<not>e s0 > 0 \<Longrightarrow> P s0 s tr \<Longrightarrow> wait_c e P s0 s tr"
+
+inductive wait_cg :: "pname \<Rightarrow> 'a eexp \<Rightarrow> 'a gassn2 \<Rightarrow> 'a gassn2" where
+  "e (the (gs0 pn)) > 0 \<Longrightarrow> P gs0 gs tr \<Longrightarrow> wait_cg pn e P gs0 gs (WaitBlockP (e (the (gs0 pn))) (\<lambda>_. gs0) ({}, {}) # tr)"
+| "\<not>e (the (gs0 pn)) > 0 \<Longrightarrow> P gs0 gs tr \<Longrightarrow> wait_cg pn e P gs0 gs tr"
+
+lemma single_assn_wait:
+  "single_assn pn (wait_c e P) = wait_cg pn e (single_assn pn P)"
+  apply (rule ext) apply (rule ext) apply (rule ext)
+  subgoal for gs0 gs tr
+    apply (rule iffI)
+    subgoal apply (elim single_assn.cases) apply auto
+      subgoal for s0 s tr'
+        apply (cases "e s0 > 0")
+        subgoal premises pre
+        proof -
+          have es0: "e s0 = e (the ((State pn s0) pn))"
+            by auto
+          then show ?thesis
+            using pre apply (elim wait_c.cases) apply auto[2]
+            apply (subst es0) apply (rule wait_cg.intros(1))
+            by (auto intro: single_assn.intros)
+        qed
+        subgoal premises pre
+        proof -
+          have es0: "e s0 = e (the ((State pn s0) pn))"
+            by auto
+          then show ?thesis
+            using pre apply (elim wait_c.cases) apply auto[1]
+            apply (rule wait_cg.intros(2))
+            by (auto intro: single_assn.intros)
+        qed
+        done
+      done
+    subgoal apply (elim wait_cg.cases) apply auto
+      subgoal for tr'
+        apply (elim single_assn.cases) apply auto
+        subgoal for s0' s' tr''
+          apply (subst ptrace_of.simps[symmetric])
+          apply (rule single_assn.intros)
+          apply (rule wait_c.intros) by auto
+        done
+      subgoal
+        apply (elim single_assn.cases) apply auto
+        subgoal for s0' s' tr''
+          apply (rule single_assn.intros)
+          apply (rule wait_c.intros) by auto
+        done
+      done
+    done
+  done
+
+lemma spec_of_wait:
+  "spec_of (Wait e) (wait_c e init)"
+  unfolding Valid_def spec_of_def init_def
+  apply (auto elim!: waitE)
+   apply (rule wait_c.intros(1)) apply auto
+  apply (rule wait_c.intros(2)) by auto
+
+lemma Valid_wait_sp:
+  assumes "spec_of c Q"
+  shows "spec_of (Wait e; c) (wait_c e Q)"
+  using assms unfolding Valid_def spec_of_def init_def
+  apply (auto elim!: seqE waitE)
+   apply (rule wait_c.intros(1)) apply auto
+  apply (rule wait_c.intros(2)) by auto
+
+inductive true_assn2 :: "'a assn2" where
+  "true_assn2 s0 s tr"
+
+text \<open>Trace is compatible with a given set of procedure names\<close>
+inductive proc_set_trace :: "pname set \<Rightarrow> 'a ptrace \<Rightarrow> bool" where
+  "proc_set_trace pns []"
+| "proc_set_trace pns tr \<Longrightarrow> proc_set_trace pns (CommBlockP ctype ch v # tr)"
+| "proc_set_trace pns tr \<Longrightarrow> \<forall>t. proc_set (p t) = pns \<Longrightarrow>
+   proc_set_trace pns (WaitBlockP d p rdy # tr)"
+
+inductive_cases proc_set_trace_waitE: "proc_set_trace pns (WaitBlockP d p rdy # tr)"
+thm proc_set_trace_waitE
+
+lemma proc_set_trace_tl:
+  "proc_set_trace pns (blk # tr) \<Longrightarrow> proc_set_trace pns tr"
+  apply (induct rule: proc_set_trace.cases)
+  by auto
+
+lemma proc_set_trace_wait:
+  "proc_set_trace pns (WaitBlockP d p rdy # tr) \<Longrightarrow> proc_set (p t) = pns"
+  apply (elim proc_set_trace_waitE) by auto
+
+inductive true_gassn :: "pname set \<Rightarrow> 'a gassn2" where
+  "proc_set gs0 = pns \<Longrightarrow> proc_set gs = pns \<Longrightarrow> proc_set_trace pns tr \<Longrightarrow>
+   true_gassn pns gs0 gs tr"
+
+text \<open>The following two lemmas show that a trace is compatible with
+  a set of procedure names if and only if it can be created using ptrace_of.
+\<close>
+lemma proc_set_trace_single:
+  "proc_set_trace {pn} (ptrace_of pn tr)"
+proof (induction tr)
+  case Nil
+  then show ?case
+    by (auto intro: proc_set_trace.intros)
+next
+  case (Cons blk tr)
+  show ?case
+    apply (cases blk)
+    using Cons by (auto intro: proc_set_trace.intros)
+qed
+
+lemma proc_set_trace_is_single:
+  "proc_set_trace {pn} tr \<Longrightarrow> \<exists>tr'. tr = ptrace_of pn tr'"
+proof (induction tr)
+  case Nil
+  show ?case
+    apply (rule exI[where x="[]"])
+    by auto
+next
+  case (Cons blk tr)
+  have "proc_set_trace {pn} tr"
+    using Cons(2) proc_set_trace_tl by auto
+  then obtain tr' where tr': "tr = ptrace_of pn tr'"
+    using Cons(1) by auto
+  show ?case
+  proof (cases blk)
+    case (CommBlockP ctype ch v)
+    show ?thesis
+      unfolding CommBlockP
+      apply (rule exI[where x="CommBlock ctype ch v # tr'"])
+      using tr' by auto
+  next
+    case (WaitBlockP d p rdy)
+    have "proc_set_trace {pn} (WaitBlockP d p rdy # tr)"
+      using Cons(2)[unfolded WaitBlockP] by auto
+    then have "proc_set (p t) = {pn}" for t
+      using proc_set_trace_wait by blast
+    then have "\<exists>p'. p t = State pn p'" for t
+      by (metis proc_set_single_elim)
+    then obtain p' where p': "p = (\<lambda>\<tau>. State pn (p' \<tau>))"
+      by metis
+    show ?thesis
+      unfolding WaitBlockP
+      apply (rule exI[where x="WaitBlock d p' rdy # tr'"])
+      using tr' p' by auto
+  qed
+qed
+
+lemma single_assn_true:
+  "single_assn pn true_assn2 = true_gassn {pn}"
+  apply (rule ext) apply (rule ext) apply (rule ext)
+  subgoal for s0 s tr
+    apply (rule iffI)
+    subgoal apply (elim single_assn.cases)
+      apply auto apply (rule true_gassn.intros)
+      using proc_set_trace_single by auto
+    subgoal apply (elim true_gassn.cases)
+      apply clarify
+      apply (elim proc_set_single_elim)
+      apply auto
+      by (metis proc_set_trace_is_single single_assn.intros true_assn2.intros)
+    done
+  done
+
+lemma entails_assumption:
+  "P s \<Longrightarrow>\<^sub>A (IFA b THEN P ELSE true_assn2 FI) s"
+  unfolding cond_assn2_def entails_def
+  using true_assn2.intros by auto
+
+text \<open>Version of wait_in_c with assumption of immediate communication\<close>
+definition wait_in_c0 :: "cname \<Rightarrow> (real \<Rightarrow> 'a assn2) \<Rightarrow> 'a assn2" where
+  "wait_in_c0 ch P = wait_in_c ch (\<lambda>d v. IFA (\<lambda>s. d = 0) THEN P v ELSE true_assn2 FI)"
+
+definition wait_in_cg0 :: "pname \<Rightarrow> cname \<Rightarrow> (real \<Rightarrow> 'a gassn2) \<Rightarrow> 'a gassn2" where
+  "wait_in_cg0 pn ch P = wait_in_cg ch (\<lambda>d v. IFG [pn] (\<lambda>s. d = 0) THEN P v ELSE true_gassn {pn} FI)"
+
+lemma single_assn_wait_in0:
+  "single_assn pn (wait_in_c0 ch P) = wait_in_cg0 pn ch (\<lambda>v. single_assn pn (P v))"
+  unfolding wait_in_c0_def wait_in_cg0_def
+  apply (subst single_assn_wait_in)
+  unfolding single_assn_cond single_assn_true by auto
+
+lemma ex6a_sp:
+  "spec_of ex6a
+    (wait_in_c0 ch2 (\<lambda>v.
+     (wait_c (\<lambda>_. 1) (wait_out_c ch1 (\<lambda>s. val s X) (\<lambda>d. init)) {{ X := (\<lambda>_. v) }})))"
+  unfolding ex6a_def
+  apply (rule spec_of_post)
+   apply (rule Valid_receive_sp)
+   prefer 2 apply clarify
+  unfolding wait_in_c0_def
+   apply (rule wait_in_c_mono)
+   apply (rule entails_assumption)
+  apply (rule Valid_wait_sp)
+  apply (rule spec_of_send)
+  done
+
+definition ex6b :: "'a proc" where
+  "ex6b = (Wait (\<lambda>_. 1); Cm (ch1[?]X))"
+
+lemma ex6b_sp:
+  "spec_of ex6b
+    (wait_c (\<lambda>_. 1) (wait_in_c ch1 (\<lambda>d v. init {{ X := (\<lambda>_. v) }})))"
+  unfolding ex6b_def
+  apply (rule Valid_wait_sp)
+  apply (rule spec_of_receive)
+  done
+
+lemma ex6:
+  "spec_of_global
+    (Parallel (Single ''a'' ex6a)
+              {ch1}
+              (Single ''b'' ex6b))
+    Q"
+  (* Stage 1: merge ex6a_sp and ex6b_sp *)
+  apply (rule spec_of_global_post)
+   apply (rule spec_of_parallel)
+      apply (rule spec_of_single)
+      apply (rule ex6a_sp)
+     apply (rule spec_of_single)
+     apply (rule ex6b_sp)
+    apply simp apply simp
+  (* Stage 2: rewrite the assertions *)
+  apply auto subgoal for s0
+    apply (auto simp add: single_assn_wait_in0 single_assn_wait updg_subst2
+                          single_assn_wait_out single_assn_wait_in single_assn_init)
+  (* Stage 3: combine the two assertions *)
+    apply (rule entails_g_trans)
+
 
 end
